Further Elgotwork

DeBruijnSSA/BinSyntax/Rewrite/Region/Structural/Elgot.lean
@@ -8,17 +8,26 @@ variable [Φ: EffInstSet φ (Ty α) ε] [PartialOrder α] [SemilatticeSup ε] [O
 
 namespace Region
 
-def Eqv.fixpoint_def' {A B : Ty α} {Γ : Ctx α ε} {L : LCtx α} (f : Eqv φ (⟨A, ⊥⟩::Γ) ((B.coprod A)::L))
-  : Eqv φ (⟨A, ⊥⟩::Γ) (B::L) := letc A nil (f.vwk1.lwk1 ;; left_exit)
+def Eqv.fixpoint_def' {A B : Ty α} {Γ : Ctx α ε} {L : LCtx α}
+  {f : Eqv φ (⟨A, ⊥⟩::Γ) ((B.coprod A)::L)}
+  : fixpoint f = letc A nil (f.vwk1.lwk1 ;; left_exit)
+  := rfl
 
-theorem Eqv.letc_to_vwk1 {Γ : Ctx α ε} {L : LCtx α} {A : Ty α} {β : Eqv φ ((B, ⊥)::Γ) (A::L)} {G}
-  : letc A β G = letc (B.prod A)
-    (ret Term.Eqv.split ;; _ ⋊ β)
-    ((ret Term.Eqv.split ⋉ _ ;; assoc ;; _ ⋊ (let2 (Term.Eqv.var 0 Ctx.Var.shead) G.vwk2)).vwk1)
-  := by
-  sorry
+
+def Eqv.fixpoint_def_vwk1 {A B : Ty α} {Γ : Ctx α ε} {L : LCtx α}
+  {f : Eqv φ (⟨A, ⊥⟩::Γ) ((B.coprod A)::L)}
+  : fixpoint f = letc A nil (f.lwk1 ;; left_exit).vwk1
+  := by rw [vwk1_seq, vwk1_lwk1]; rfl
+
+-- theorem Eqv.letc_to_vwk1 {Γ : Ctx α ε} {L : LCtx α} {A : Ty α} {β : Eqv φ ((B, ⊥)::Γ) (A::L)} {G}
+--   : letc A β G = letc (B.prod A)
+--     (ret Term.Eqv.split ;; _ ⋊ β)
+--     ((ret Term.Eqv.split ⋉ _ ;; assoc ;; _ ⋊ (let2 (Term.Eqv.var 0 Ctx.Var.shead) G.vwk2)).vwk1)
+--   := by
+--   sorry
 
 theorem Eqv.letc_vwk1_den {Γ : Ctx α ε}
   {A B : Ty α} {β : Eqv φ ((X, ⊥)::Γ) [A, B]} {G : Eqv φ ((A, ⊥)::Γ) [A, B]}
-  : letc A β G.vwk1 = β.packed_out ;; fixpoint (coprod (coprod zero inj_l) (G.packed_out ;; inj_r))
+  : letc A β G.vwk1 = (β.packed_out ;; sum (coprod zero nil) nil) ;;
+                    coprod nil (fixpoint (G.packed_out ;; coprod (coprod zero inj_l) inj_r))
   := sorry
